src/case_study/examples.v
@@ -1,0 +1,129 @@
+From iris.base_logic Require Export gen_heap.
+From iris.algebra Require Export list excl_auth.
+From nextgen.case_study.program_logic Require Import CC_ectx_lifting
+     CC_ectxi_language CC_ectx_lifting weakestpre.
+From nextgen.case_study Require Export stack_lang stack_transform rules_unary.
+From iris.proofmode Require Import tactics.
+From stdpp Require Import fin_maps.
+From nextgen Require Import nextgen_basic gen_trans gmap_view_transformation nextgen_pointwise nextgen_id.
+
+From nextgen.case_study Require Import stack_lang_notation.
+
+Set Default Proof Using "Type".
+Import uPred.
+
+Lemma fill_inner_cons n e K Ks :
+  fill (K :: Ks) (n,e) = fill Ks (n, fill_item K e).
+Proof. auto. Qed.
+
+Ltac peel_ctx := rewrite fill_inner_cons;simpl fill_item.
+
+Ltac prepare_ctx :=
+  (try rewrite /stack_fill_item /=) ;match goal with
+  | |- context [ WP (?n,?e) @ _ ; _ {{ _ }}%I ] =>
+      rewrite (construct_ctx_eq n e);simpl app;
+      peel_ctx
+  end.
+
+Section examples.
+  Open Scope expr_scope.
+
+  Definition example1 : expr :=
+    (λ: global, "k", "y", let: "x" := sref 42 in !"x") ().
+
+  Definition example2 : expr :=
+    (λ: global, "<>", "f", let: "y" := sref 42 in "f" ("y")) (λ: global, "<>", "x", !"x").
+
+  Definition example3 : expr :=
+    let: "g" := λ: global, "<>", "f'", "f'" () in
+    let: "f" := λ: global, "<>", "<>", let: "x" := sref 42 in "g" (λ: local 0, "<>", "<>", !"x") in
+    "f" ().    
+    
+  
+  Definition stuck_example : expr :=
+    ! ((λ: global, "<>", "<>", sref 42) ()).
+
+End examples.
+
+Section stack_lang_examples.
+  Context `{heapGS Σ}.
+
+
+  Lemma example1_spec :
+    {{{ [size] 0 }}} (0,example1) {{{ v, RET v; ⌜v.2 = NatV 42⌝ }}}.
+  Proof.
+    iIntros (Φ) "Hsize #HΦ /=". rewrite /example1. prepare_ctx.
+    iApply wp_call_global;[eauto|iFrame]. iNext. iIntros "Hsize /=". prepare_ctx.
+    iApply wp_stack_alloc;[lia|repeat constructor|iFrame].
+    iNext. iIntros (l) "[Hsize Hl]". peel_ctx.
+    iApply wp_LetIn. iNext. simpl subst'.
+    iApply wp_stack_load;[constructor;lia|iFrame].
+    iNext. iIntros "[Hsize Hl]". peel_ctx.
+    iApply wp_return;[lia..|iFrame]. iNext. iIntros "Hsize".
+    simpl. iModIntro. iApply wp_value. iApply "HΦ". simpl. auto.
+  Qed.
+
+  Lemma example2_spec :
+    {{{ [size] 0 }}} (0,example2) {{{ v, RET v; ⌜v.2 = NatV 42⌝ }}}.
+  Proof.
+    iIntros (Φ) "Hsize #HΦ /=". rewrite /example2. prepare_ctx.
+    iApply wp_call_global;[eauto|iFrame]. iNext. iIntros "Hsize /=". prepare_ctx.
+    iApply wp_stack_alloc;[lia|repeat constructor|iFrame].
+    iNext. iIntros (l) "[Hsize Hl]". peel_ctx.
+    iApply wp_LetIn. iNext. simpl subst'.
+    iApply wp_call_global;[eauto|iFrame]. iNext. iIntros "Hsize /=".
+    prepare_ctx.
+    iApply wp_stack_load;[constructor;lia|iFrame].
+    iNext. iIntros "[Hsize Hl]". peel_ctx.
+    iApply wp_return;[lia..|iFrame]. iNext. iIntros "Hsize /=".
+    iDestruct (stack_stack_pop_intro _ _ _ _ 1 with "Hl") as "Hl";[lia|].
+    iDestruct (stack_size_frag_stack_pop _ 1 with "Hsize") as "Hsize".
+    iModIntro. prepare_ctx.
+    iApply wp_return;[lia..|iFrame]. iNext. iIntros "Hsize /=".
+    iModIntro. iApply wp_value. iApply "HΦ";auto.
+  Qed.
+
+  Lemma example3_spec :
+    {{{ [size] 0 }}} (0,example3) {{{ v, RET v; ⌜v.2 = NatV 42⌝ }}}.
+  Proof.
+    iIntros (Φ) "Hsize #HΦ /=". rewrite /example2. prepare_ctx.
+    iApply wp_LetIn. iNext. simpl subst'.
+    iApply wp_LetIn. iNext. simpl subst'.
+    iApply wp_call_global;[eauto|iFrame]. iNext. iIntros "Hsize /=". prepare_ctx.
+    iApply wp_stack_alloc;[lia|repeat constructor|iFrame]. iNext. iIntros (l) "[Hsize Hl]". peel_ctx.
+    iApply wp_LetIn. iNext. simpl subst'.
+    iApply wp_call_global;[eauto|iFrame]. iNext. iIntros "Hsize /=". prepare_ctx.
+    iApply wp_call_local;[eauto..|iFrame];[constructor;lia|]. simpl. prepare_ctx.
+    iNext. iIntros "Hsize".
+    (* NOTE: the local stack pointer has been shifted to point two frame down *)
+    iApply wp_stack_load;[constructor;lia|iFrame]. iNext. iIntros "[Hsize Hl]". peel_ctx.
+    iApply wp_return;[lia..|]. iFrame. iNext. iIntros "Hsize /=".
+    iDestruct (stack_size_frag_stack_pop _ 2 with "Hsize") as "Hsize".
+    iModIntro. prepare_ctx.
+    iApply wp_return;[lia..|]. iFrame. iNext. iIntros "Hsize /=".
+    iDestruct (stack_size_frag_stack_pop _ 1 with "Hsize") as "Hsize".
+    iModIntro. prepare_ctx.
+    iApply wp_return;[lia..|]. iFrame. iNext. iIntros "Hsize /=".
+    iModIntro. iApply wp_value. iApply "HΦ";auto.
+  Qed.
+
+  (* The following lemma cannot be proved, since the program will get
+  stuck once the caller tried to load the callee's now popped stack
+  location *)
+  Lemma stuck_example_failed_spec :
+    {{{ [size] 1 }}} (1,stuck_example) {{{ v, RET v; False }}}.
+  Proof.
+    iIntros (Φ) "Hsize #HΦ /=". rewrite /stuck_example. prepare_ctx.
+    iApply wp_call_global;[eauto|iFrame]. iNext. iIntros "Hsize /=". prepare_ctx.
+    iApply wp_stack_alloc;[lia|repeat constructor|iFrame]. iNext. iIntros (l) "[Hsize Hl]". peel_ctx.
+    iApply wp_return;[lia..|iFrame]. iNext. iIntros "Hsize /=".
+    iModIntro.
+    (* STUCK! the points-to for l gets lost, its lifetime is not less than 1 *)
+  Abort.
+
+  
+  
+
+End stack_lang_examples.
+
+
