src/case_study/stack_lang_notation.v
@@ -1,0 +1,184 @@
+From nextgen.case_study.program_logic Require Import weakestpre CC_ectx_language.
+From nextgen.case_study Require Export stack_lang.
+From iris.prelude Require Export options.
+From stdpp Require Export pretty strings binders.
+
+Global Instance pretty_loc : Pretty loc := string_of_pos.
+
+Global Instance pretty_binder : Pretty binder :=
+  λ b, match b with
+       | BNamed x => x
+       | BAnon => "<>"
+       end.
+
+Global Instance pretty_tag : Pretty tag :=
+  λ t, match t with
+       | global => "global"
+       | borrow => "borrow"
+       | local i => "local " +:+ pretty i
+       end.
+
+(** Note that this instance does not print function bodies or continuation contexts and is thus not
+injective (unlike most `pretty` instances). *)
+Global Instance pretty_val : Pretty val :=
+  fix go v :=
+    match v with
+    | ContV i K => "Cont " +:+ pretty i +:+ "[<ctx>]"
+    | LocV δ l => "#v" +:+ "[" +:+ pretty δ +:+ ", " +:+ pretty l +:+ "]"
+    | NatV n => "#v" +:+ pretty n
+    | BoolV b => "#v" +:+ if b then "true" else "false"
+    | UnitV => "#v()"
+    | LamV δ k x e => "λ: " +:+ pretty δ +:+ ", " +:+ pretty k +:+ ", " +:+ pretty x +:+ ", <body>"
+    | PairV v1 v2 => "<" +:+ go v1 +:+ ", " +:+ go v2 +:+ ">"
+    end.
+
+Global Instance pretty_bin_op : Pretty binop :=
+  λ op, match op with
+        | Sub => "-"
+        | Le => "≤"
+        | Lt => "<"
+        | Eq => "="
+        | _ => "+"
+        end.
+
+Definition LocT : Type := tag * loc.
+Definition LocP (p: LocT) : expr := Loc p.1 p.2.
+
+(** Coercions to make programs easier to type. *)
+Coercion Nat : nat >-> expr.
+Coercion Bool : bool >-> expr.
+Coercion Var : string >-> expr.
+Coercion Call : expr >-> Funclass.
+Coercion LocP : LocT >-> expr.
+(** Define some derived forms. *)
+Notation Seq e1 e2 := (LetIn BAnon e1 e2) (only parsing).
+Notation SeqCtx e2 := (LetInCtx BAnon e2) (only parsing).
+
+(* No scope for the values, does not conflict and scope is often not inferred
+properly. *)
+Notation "# ( δ , l )" := (LocV δ l%Z%V%stdpp) (at level 8, format "# ( δ , l )").
+
+(** Syntax inspired by Coq/Ocaml. Constructions with higher precedence come
+    first. *)
+Notation "< e1 , e2 , .. , en >" := (Pair .. (Pair e1 e2) .. en) : expr_scope.
+Notation "< e1 , e2 , .. , en >" := (PairV .. (PairV e1 e2) .. en) : val_scope.
+
+Notation "()" := lang.Unit : expr_scope.
+Notation "! e" := (Load e%E) (at level 9, right associativity) : expr_scope.
+Notation "'href' e" := (Halloc e%E) (at level 10) : expr_scope.
+Notation "'sref' e" := (Salloc e%E) (at level 10) : expr_scope.
+
+Notation "e1 + e2" := (BinOp Add e1%E e2%E) : expr_scope.
+Notation "e1 - e2" := (BinOp Sub e1%E e2%E) : expr_scope.
+
+Notation "e1 ≤ e2" := (BinOp Le e1%E e2%E) : expr_scope.
+Notation "e1 < e2" := (BinOp Lt e1%E e2%E) : expr_scope.
+Notation "e1 = e2" := (BinOp Eq e1%E e2%E) : expr_scope.
+
+(* The unicode ← is already part of the notation "_ ← _; _" for bind. *)
+Notation "e1 <- e2" := (Store e1%E e2%E) (at level 80) : expr_scope.
+
+(* The breaking point '/  ' makes sure that the body of the rec is indented
+by two spaces in case the whole rec does not fit on a single line. *)
+Notation "'if:' e1 'then' e2 'else' e3" := (If e1%E e2%E e3%E)
+                                             (at level 200, e1, e2, e3 at level 200) : expr_scope.
+
+(* Shortcircuit Boolean connectives *)
+Notation "e1 && e2" :=
+  (If e1%E e2%E (Bool false)) (only parsing) : expr_scope.
+Notation "e1 || e2" :=
+  (If e1%E (Bool true) e2%E) (only parsing) : expr_scope.
+
+(* The breaking point '/  ' makes sure that the body of the λ: is indented
+by two spaces in case the whole λ: does not fit on a single line. *)
+(* | Lam (δ : tag) (k x : binder) (e : expr)*)
+Notation "λ: δ , k , x , e" := (Lam δ k%binder x%binder e%E)
+  (at level 200, x at level 1, e at level 200,
+   format "'[' 'λ:'  δ ,  k ,  x ,  '/  ' e ']'") : expr_scope.
+Notation "λ: δ , k , x y .. z , e" := (Lam δ k%binder x%binder (Lam δ k%binder y%binder .. (Lam δ k%binder z%binder e%E) ..))
+  (at level 200, x, y, z at level 1, e at level 200,
+    format "'[' 'λ:'  δ ,  k ,  x  y  ..  z ,  '/  ' e ']'") : expr_scope.
+
+Notation "λ: δ , k , x , e" := (LamV δ k%binder x%binder e%E)
+  (at level 200, x at level 1, e at level 200,
+   format "'[' 'λ:'  δ ,  k ,  x ,  '/  ' e ']'") : val_scope.
+Notation "λ: δ , k , x y .. z , e" := (LamV δ k%binder x%binder (LamV δ k%binder y%binder .. (LamV δ k%binder z%binder e%E) ..))
+  (at level 200, x, y, z at level 1, e at level 200,
+   format "'[' 'λ:'  δ ,  k ,  x  y  ..  z ,  '/  ' e ']'") : val_scope.
+
+Notation "'let:' x := e1 'in' e2" := (LetIn x%binder e1%E e2%E)
+  (at level 200, x at level 1, e1, e2 at level 200,
+   format "'[' 'let:'  x  :=  '[' e1 ']'  'in'  '/' e2 ']'") : expr_scope.
+Notation "e1 ;; e2" := (Seq e1%E e2%E)
+  (at level 100, e2 at level 200,
+    format "'[' '[hv' '[' e1 ']' ;;  ']' '/' e2 ']'") : expr_scope.
+
+(* Overloading the bi notation of Texan triples such that the postcondition is wrapped in a plainly *)
+Notation "'{{{' P } } } e @ s ; E {{{ x .. y , 'RET' pat ; Q } } }" :=
+  (□ ∀ Φ,
+      P -∗ ▷ ■ (∀ x, .. (∀ y, Q -∗ Φ pat%V) .. ) -∗ WP e @ s; E {{ Φ }})%I
+    (at level 20, x closed binder, y closed binder,
+     format "'[hv' {{{  '[' P  ']' } } }  '/  ' e  '/' @  '[' s ;  '/' E  ']' '/' {{{  '[' x  ..  y ,  RET  pat ;  '/' Q  ']' } } } ']'") : bi_scope.
+Notation "'{{{' P } } } e @ E {{{ x .. y , 'RET' pat ; Q } } }" :=
+  (□ ∀ Φ,
+      P -∗ ▷ ■ (∀ x, .. (∀ y, Q -∗ Φ pat%V) .. ) -∗ WP e @ E {{ Φ }})%I
+    (at level 20, x closed binder, y closed binder,
+     format "'[hv' {{{  '[' P  ']' } } }  '/  ' e  '/' @  E  '/' {{{  '[' x  ..  y ,  RET  pat ;  '/' Q  ']' } } } ']'") : bi_scope.
+Notation "'{{{' P } } } e @ E ? {{{ x .. y , 'RET' pat ; Q } } }" :=
+  (□ ∀ Φ,
+      P -∗ ▷ ■ (∀ x, .. (∀ y, Q -∗ Φ pat%V) .. ) -∗ WP e @ E ?{{ Φ }})%I
+    (at level 20, x closed binder, y closed binder,
+     format "'[hv' {{{  '[' P  ']' } } }  '/  ' e  '/' @  E  '/' ? {{{  '[' x  ..  y ,  RET  pat ;  '/' Q  ']' } } } ']'") : bi_scope.
+Notation "'{{{' P } } } e {{{ x .. y , 'RET' pat ; Q } } }" :=
+  (□ ∀ Φ,
+      P -∗ ▷ ■ (∀ x, .. (∀ y, Q -∗ Φ pat%V) .. ) -∗ WP e {{ Φ }})%I
+    (at level 20, x closed binder, y closed binder,
+     format "'[hv' {{{  '[' P  ']' } } }  '/  ' e  '/' {{{  '[' x  ..  y ,  RET  pat ;  '/' Q  ']' } } } ']'") : bi_scope.
+Notation "'{{{' P } } } e ? {{{ x .. y , 'RET' pat ; Q } } }" :=
+  (□ ∀ Φ,
+      P -∗ ▷ ■ (∀ x, .. (∀ y, Q -∗ Φ pat%V) .. ) -∗ WP e ?{{ Φ }})%I
+    (at level 20, x closed binder, y closed binder,
+     format "'[hv' {{{  '[' P  ']' } } }  '/  ' e  '/' ? {{{  '[' x  ..  y ,   RET  pat ;  '/' Q  ']' } } } ']'") : bi_scope.
+
+Notation "'{{{' P } } } e @ s ; E {{{ 'RET' pat ; Q } } }" :=
+  (□ ∀ Φ, P -∗ ▷ ■ (Q -∗ Φ pat%V) -∗ WP e @ s; E {{ Φ }})%I
+    (at level 20,
+     format "'[hv' {{{  '[' P  ']' } } }  '/  ' e  '/' @  '[' s ;  '/' E  ']' '/' {{{  '[' RET  pat ;  '/' Q  ']' } } } ']'") : bi_scope.
+Notation "'{{{' P } } } e @ E {{{ 'RET' pat ; Q } } }" :=
+  (□ ∀ Φ, P -∗ ▷ ■ (Q -∗ Φ pat%V) -∗ WP e @ E {{ Φ }})%I
+    (at level 20,
+     format "'[hv' {{{  '[' P  ']' } } }  '/  ' e  '/' @  E  '/' {{{  '[' RET  pat ;  '/' Q  ']' } } } ']'") : bi_scope.
+Notation "'{{{' P } } } e @ E ? {{{ 'RET' pat ; Q } } }" :=
+  (□ ∀ Φ, P -∗ ▷ ■ (Q -∗ Φ pat%V) -∗ WP e @ E ?{{ Φ }})%I
+    (at level 20,
+     format "'[hv' {{{  '[' P  ']' } } }  '/  ' e  '/' @  E  '/' ? {{{  '[' RET  pat ;  '/' Q  ']' } } } ']'") : bi_scope.
+Notation "'{{{' P } } } e {{{ 'RET' pat ; Q } } }" :=
+  (□ ∀ Φ, P -∗ ▷ ■ (Q -∗ Φ pat%V) -∗ WP e {{ Φ }})%I
+    (at level 20,
+     format "'[hv' {{{  '[' P  ']' } } }  '/  ' e  '/' {{{  '[' RET  pat ;  '/' Q  ']' } } } ']'") : bi_scope.
+Notation "'{{{' P } } } e ? {{{ 'RET' pat ; Q } } }" :=
+  (□ ∀ Φ, P -∗ ▷ ■ (Q -∗ Φ pat%V) -∗ WP e ?{{ Φ }})%I
+    (at level 20,
+     format "'[hv' {{{  '[' P  ']' } } }  '/  ' e  '/' ? {{{  '[' RET  pat ;  '/' Q  ']' } } } ']'") : bi_scope.
+
+(** Aliases for stdpp scope -- they inherit the levels and format from above. *)
+Notation "'{{{' P } } } e @ s ; E {{{ x .. y , 'RET' pat ; Q } } }" :=
+  (∀ Φ, P -∗ ▷ ■ (∀ x, .. (∀ y, Q -∗ Φ pat%V) .. ) -∗ WP e @ s; E {{ Φ }}) : stdpp_scope.
+Notation "'{{{' P } } } e @ E {{{ x .. y , 'RET' pat ; Q } } }" :=
+  (∀ Φ, P -∗ ▷ ■ (∀ x, .. (∀ y, Q -∗ Φ pat%V) .. ) -∗ WP e @ E {{ Φ }}) : stdpp_scope.
+Notation "'{{{' P } } } e @ E ? {{{ x .. y , 'RET' pat ; Q } } }" :=
+  (∀ Φ, P -∗ ▷ ■ (∀ x, .. (∀ y, Q -∗ Φ pat%V) .. ) -∗ WP e @ E ?{{ Φ }}) : stdpp_scope.
+Notation "'{{{' P } } } e {{{ x .. y , 'RET' pat ; Q } } }" :=
+  (∀ Φ, P -∗ ▷ ■ (∀ x, .. (∀ y, Q -∗ Φ pat%V) .. ) -∗ WP e {{ Φ }}) : stdpp_scope.
+Notation "'{{{' P } } } e ? {{{ x .. y , 'RET' pat ; Q } } }" :=
+  (∀ Φ, P -∗ ▷ ■ (∀ x, .. (∀ y, Q -∗ Φ pat%V) .. ) -∗ WP e ?{{ Φ }}) : stdpp_scope.
+Notation "'{{{' P } } } e @ s ; E {{{ 'RET' pat ; Q } } }" :=
+  (∀ Φ, P -∗ ▷ ■ (Q -∗ Φ pat%V) -∗ WP e @ s; E {{ Φ }}) : stdpp_scope.
+Notation "'{{{' P } } } e @ E {{{ 'RET' pat ; Q } } }" :=
+  (∀ Φ, P -∗ ▷ ■ (Q -∗ Φ pat%V) -∗ WP e @ E {{ Φ }}) : stdpp_scope.
+Notation "'{{{' P } } } e @ E ? {{{ 'RET' pat ; Q } } }" :=
+  (∀ Φ, P -∗ ▷ ■ (Q -∗ Φ pat%V) -∗ WP e @ E ?{{ Φ }}) : stdpp_scope.
+Notation "'{{{' P } } } e {{{ 'RET' pat ; Q } } }" :=
+  (∀ Φ, P -∗ ▷ ■ (Q -∗ Φ pat%V) -∗ WP e {{ Φ }}) : stdpp_scope.
+Notation "'{{{' P } } } e ? {{{ 'RET' pat ; Q } } }" :=
+  (∀ Φ, P -∗ ▷ ■ (Q -∗ Φ pat%V) -∗ WP e ?{{ Φ }}) : stdpp_scope.
